Sorting/Test.v
@@ -22,130 +22,130 @@ Set Implicit Arguments.
 
 (* Slow sorts on small lists. *)
 
-(*Time Compute ss natle (cycle 100 testl).
-Time Compute ss' natle (cycle 100 testl).
-Time Compute ss'' natle (cycle 100 testl).
-Time Compute ss_bifilter natle (cycle 500 testl).
+(*Time Compute ss natlt (cycle 100 testl).
+Time Compute ss' natlt (cycle 100 testl).
+Time Compute ss'' natlt (cycle 100 testl).
+Time Compute ss_bifilter natlt (cycle 500 testl).
 Time Compute ss_mins' natlt (cycle 500 testl).
 
-Time Compute ss natle (cycle 10 testl).
-Time Compute insertionSort natle (cycle 10 testl).*)
+Time Compute ss natlt (cycle 10 testl).
+Time Compute insertionSort natlt (cycle 10 testl).*)
 
 (* Fast sorts on medium lists. *)
 
-(*Time Compute ms natle (cycle 100 testl).
-Time Compute ms2 natle (cycle 100 testl).
+(*Time Compute ms natlt (cycle 100 testl).
+Time Compute ms2 natlt (cycle 100 testl).
 
-Time Compute qs natle (cycle 100 testl).
-Time Compute qs2 natle (cycle 100 testl).
+Time Compute qs natlt (cycle 100 testl).
+Time Compute qs2 natlt (cycle 100 testl).
 
 Time Compute tqs natlt (cycle 100 testl).
 
-Time Compute treeSort natle (cycle 100 testl).
-Time Compute treeSort' natle (cycle 100 testl).
+Time Compute treeSort natlt (cycle 100 testl).
+Time Compute treeSort' natlt (cycle 100 testl).
 
-Time Compute redblackSort natle (cycle 100 testl).
-(*Time Compute redblackSort' natle (cycle 100 testl).*)
+Time Compute redblackSort natlt (cycle 100 testl).
+(*Time Compute redblackSort' natlt (cycle 100 testl).*)
 
-Time Eval lazy in leftistHeapsort natle (cycle 100 testl).
-(*Time Eval lazy in leftistHeapsort' natle (cycle 100 testl).*)
-Time Compute leftistHeapsort3 natle (cycle 100 testl).
+Time Eval lazy in leftistHeapsort natlt (cycle 100 testl).
+(*Time Eval lazy in leftistHeapsort' natlt (cycle 100 testl).*)
+Time Compute leftistHeapsort3 natlt (cycle 100 testl).
 
-Time Eval lazy in splaySort natle (cycle 100 testl).
+Time Eval lazy in splaySort natlt (cycle 100 testl).
 
-Time Eval lazy in pairingSort natle (cycle 100 testl).
+Time Eval lazy in pairingSort natlt (cycle 100 testl).
 
 *)
 
 (* Fast sorts on big lists. *)
 
 (*
-Time Compute ms natle (cycle 200 testl).
-Time Compute ms2 natle (cycle 200 testl).
-Time Compute ums_wut (Small_recdepth natle 0) (redblackSort natle)
-                     (MsSplit natle) (cycle 200 testl).
-Time Compute trollms 1 (redblackSort natle) (MsSplit natle)
+Time Compute ms natlt (cycle 200 testl).
+Time Compute ms2 natlt (cycle 200 testl).
+Time Compute ums_wut (Small_recdepth natlt 0) (redblackSort natle)
+                     (MsSplit natlt) (cycle 200 testl).
+Time Compute trollms 1 (redblackSort natlt) (MsSplit natle)
                (cycle 200 testl).
 
 
-Time Compute qs natle (cycle 200 testl).
-Time Compute qs2 natle (cycle 200 testl).
-Time Compute ums 0 1 (treeSort natle) (MsSplit natle) (cycle 500 testl).
+Time Compute qs natlt (cycle 200 testl).
+Time Compute qs2 natlt (cycle 200 testl).
+Time Compute ums 0 1 (treeSort natlt) (MsSplit natle) (cycle 500 testl).
 *)
 
 (*
-Time Compute treeSort natle (cycle 1000 testl).
-Time Compute treeSort' natle (cycle 1000 testl).
+Time Compute treeSort natlt (cycle 1000 testl).
+Time Compute treeSort' natlt (cycle 1000 testl).
 *)
 
 (*
-Time Compute redblackSort natle (cycle 1000 testl).
+Time Compute redblackSort natlt (cycle 1000 testl).
 
-Time Compute hqs 64 (Sort_redblackSort natle) (cycle 1000 testl).
+Time Compute hqs 64 (Sort_redblackSort natlt) (cycle 1000 testl).
 
-Time Eval lazy in leftistHeapsort' natle (cycle 300 testl).
+Time Eval lazy in leftistHeapsort' natlt (cycle 300 testl).
 *)
 
 (* Hybrid mergesort on big lists. *)
-(*Time Compute @ghms 512 natle (insertionSort natle) (MsSplit natle)
+(*Time Compute @ghms 512 natlt (insertionSort natle) (MsSplit natle)
   (cycle 200 testl).
 
-Time Compute @ghms 1024 natle (treeSort natle) (MsSplit natle)
+Time Compute @ghms 1024 natlt (treeSort natle) (MsSplit natle)
   (cycle 200 testl).
 
-Time Compute @ghms 1024 natle (redblackSort natle) (MsSplit natle)
+Time Compute @ghms 1024 natlt (redblackSort natle) (MsSplit natle)
   (cycle 200 testl). *)
 
 (* Bad
-Time Compute @ghms 1024 natle (leftistHeapsort' natle) (MsSplit natle)
+Time Compute @ghms 1024 natlt (leftistHeapsort' natle) (MsSplit natle)
   (cycle 200 testl).
 *)
 
-(*Time Compute @hqs 1024 natle (insertionSort natle) (cycle 200 testl).
+(*Time Compute @hqs 1024 natlt (insertionSort natle) (cycle 200 testl).
 
-Time Compute @hqs 512 natle (treeSort natle) (cycle 200 testl).
+Time Compute @hqs 512 natlt (treeSort natle) (cycle 200 testl).
 
-Time Compute @hqs 512 natle (redblackSort natle) (cycle 200 testl).
+Time Compute @hqs 512 natlt (redblackSort natle) (cycle 200 testl).
 *)
 
 (* Bad
-  Time Compute @hqs 256 natle (leftistHeapsort natle) (cycle 200 testl).
+  Time Compute @hqs 256 natlt (leftistHeapsort natle) (cycle 200 testl).
 *)
 
-(*Time Compute @htqs 1 natlt (insertionSort natle) (cycle 200 testl).
+(*Time Compute @htqs 1 natlt (insertionSort natlt) (cycle 200 testl).
 
-Time Compute @htqs 1 natlt (treeSort natle) (cycle 200 testl).
+Time Compute @htqs 1 natlt (treeSort natlt) (cycle 200 testl).
 
-Time Compute @htqs 1 natlt (redblackSort natle) (cycle 200 testl).*)
+Time Compute @htqs 1 natlt (redblackSort natlt) (cycle 200 testl).*)
 
 (* Long lists made of one element. *)
 Definition l1 := cycle 2500 [0].
 
 (*
-Time Compute @ghms 64 natle (insertionSort natle) (MsSplit natle) l1.
+Time Compute @ghms 64 natlt (insertionSort natle) (MsSplit natle) l1.
 
-Time Compute @ghms 64 natle (treeSort natle) (MsSplit natle) l1.
-Time Compute @ghms 64 natle (redblackSort natle) (MsSplit natle) l1.
+Time Compute @ghms 64 natlt (treeSort natle) (MsSplit natle) l1.
+Time Compute @ghms 64 natlt (redblackSort natle) (MsSplit natle) l1.
 
-Time Compute @ghms 64 natle (pairingSort natle) (MsSplit natle) l1.
+Time Compute @ghms 64 natlt (pairingSort natle) (MsSplit natle) l1.
 
-Time Compute @hqs 1024 natle (Sort_insertionSort natle) l1.
+Time Compute @hqs 1024 natlt (Sort_insertionSort natle) l1.
 *)
 
-(*Time Compute @hqs 512 natle (Sort_treeSort natle) l1.*)
+(*Time Compute @hqs 512 natlt (Sort_treeSort natle) l1.*)
 
 (*
-Time Compute @hqs 512 natle (Sort_redblackSort natle) l1.
+Time Compute @hqs 512 natlt (Sort_redblackSort natle) l1.
 
-Time Compute @hqs 512 natle (Sort_pairingSort natle) l1.
+Time Compute @hqs 512 natlt (Sort_pairingSort natle) l1.
 *)
 
 (*
-Time Compute @htqs 0 natlt (insertionSort natle) l1.
+Time Compute @htqs 0 natlt (insertionSort natlt) l1.
 
-Time Compute @htqs 0 natlt (treeSort natle) l1.
+Time Compute @htqs 0 natlt (treeSort natlt) l1.
 
-Time Compute @htqs 0 natlt (redblackSort natle) l1.
+Time Compute @htqs 0 natlt (redblackSort natlt) l1.
 
 Time Compute @uqs natlt (Small_head natlt) (AdHocSort_id natlt)
                  (Pivot_head natlt) (Partition_trifilter natlt) l1.
@@ -160,12 +160,12 @@ end.
 (*CoFixpoint rand (seed n1 n2 : Z) : Stream Z :=
 let seed' := Zmod seed n2 in Cons seed' (rand (seed' * n1) n1 n2).*)
 
-(*Time Compute qs natle (toN 500).
+(*Time Compute qs natlt (toN 500).
 Time Compute tqs natlt (toN 200).*)
 
-(*Time Compute insertionSort natle (toN 500).
+(*Time Compute insertionSort natlt (toN 500).
 
-Time Compute treeSort natle (toN 500).
-Time Compute redblackSort natle (toN 500).
+Time Compute treeSort natlt (toN 500).
+Time Compute redblackSort natlt (toN 500).
 
-Time Compute pairingSort natle (toN 500).*)
+Time Compute pairingSort natlt (toN 500).*)
